Prove lemmas about set-related transforms

fiat2/src/fiat2/CollectionTransf.v
@@ -10,6 +10,12 @@ Definition annotate_collection (e : expr) : expr :=
       if (negb (v =? acc) && (v =? v') && (acc =? acc'))%bool then EACFold AGSum (EBagOf l)
       else e
   | EUnop OLength l => EACFold AGCount (EBagOf l)
+  | EFold l (EAtom (ANone None)) v0 acc0
+      (EOptMatch (EVar acc1) (EUnop OSome (EVar v1))
+         x0 (EIf (EBinop OLess (EVar v2) (EVar x1)) (EUnop OSome (EVar v3)) (EVar acc2))) =>
+      if (all_neqb [v0; acc0; x0] && all_eqb [(v0, [v1; v2; v3]); (acc0, [acc1; acc2]); (x0, [x1])])%bool
+      then EACIFold AGMin (ESetOf l)
+      else e
   | _ => e
   end.
 
@@ -23,9 +29,20 @@ Fixpoint bag_of (e : expr) : expr :=
   | _ => EBagOf e
   end.
 
+Fixpoint set_of (e : expr) : expr :=
+  match e with
+  | EFlatmap LikeList e1 x e2 => EFlatmap LikeSet (set_of e1) x (set_of e2)
+  | EFilter LikeList e x p => EFilter LikeSet (set_of e) x p
+  | EJoin LikeList e1 e2 x y p e3 => EJoin LikeSet (set_of e1) (set_of e2) x y p e3
+  | EProj LikeList e1 x e2 => EProj LikeSet (set_of e1) x e2
+  | EBinop OCons e1 e2 => EBinop OSetInsert (set_of e2) e1
+  | _ => ESetOf e
+  end.
+
 Definition push_down_collection (e : expr) : expr :=
   match e with
   | EBagOf e => bag_of e
+  | ESetOf e => set_of e
   | _ => e
   end.
 
@@ -34,6 +51,11 @@ Definition ex : expr :=
     (EBinop OEq (EAccess (EVar "x") "attr") (EAtom (AInt 0)))).
 Compute fold_expr push_down_collection (fold_expr annotate_collection ex).
 
+Definition ex1 : expr :=
+  EFold (EProj LikeList (ELoc "tbl") "r" (EAccess (EVar "r") "attr")) (EAtom (ANone None)) "v" "acc"
+      (EOptMatch (EVar "acc") (EUnop OSome (EVar "v"))
+         "x" (EIf (EBinop OLess (EVar "v") (EVar "x")) (EUnop OSome (EVar "v")) (EVar "acc"))).
+Compute fold_expr push_down_collection (fold_expr annotate_collection ex1).
 
 Section WithWord.
   Context {width: Z} {word: word.word width}.
@@ -169,6 +191,62 @@ Section WithWord.
     Context {tenv: map.map string type} {tenv_ok: map.ok tenv}.
     Context {locals: map.map string value} {locals_ok: map.ok locals}.
 
+    Lemma set_insert_incl_r : forall (a : value) l,
+        incl (a :: l) (set_insert a l).
+      induction l; cbn.
+      1:{ constructor. destruct_In; auto.
+          apply in_nil in H; intuition idtac. }
+      repeat case_match.
+      1: apply incl_refl.
+      1:{ apply value_eqb_eq in E0; subst.
+          unfold incl; intros. destruct_In; auto.
+          left; reflexivity. }
+      1:{ apply incl_cons_inv in IHl; intuition idtac.
+          unfold incl; intros. destruct_In.
+          1: right; auto.
+          destruct_In.
+          1: left; auto.
+          1: right; auto. }
+    Qed.
+
+    Lemma list_to_set_incl_r : forall (l : list value),
+        incl l (list_to_set l).
+    Proof.
+      induction l; cbn; auto using incl_nil_l.
+      eapply incl_tran; [ apply incl_cons_step | ]; eauto.
+      apply set_insert_incl_r.
+    Qed.
+
+    Lemma aci_aggr_alt : forall f l,
+        Forall (fun v => type_of_value v TInt) l ->
+        fold_right
+          (fun v acc0 : value =>
+             match acc0 with
+             | VOption (Some (VInt v')) =>
+                 match v with
+                 | VInt v1 => VOption (Some (VInt (f v1 v')))
+                 | _ => VUnit
+                 end
+             | VOption None => VOption (Some v)
+             | _ => VUnit
+             end) (VOption None) l =
+          fold_right
+            (fun v acc0 : value =>
+               match v, acc0 with
+               | VInt v1, VOption (Some (VInt v')) =>
+                   VOption (Some (VInt (f v1 v')))
+               | VInt v1, VOption None => VOption (Some v)
+               | _, _ => VUnit
+               end) (VOption None) l.
+    Proof.
+      intros. apply In_fold_right_ext with (P:=fun _ => True); intuition idtac.
+      apply_Forall_In.
+      lazymatch goal with
+        H: type_of_value _ _ |- _ =>
+          inversion H; subst end.
+      case_match; auto.
+    Qed.
+
     Theorem annotate_collection_preserve_ty : forall e Gstore Genv t,
         type_of Gstore Genv e t ->
         type_of Gstore Genv (annotate_collection e) t.
@@ -177,12 +255,12 @@ Section WithWord.
       all: try now (econstructor; eauto).
       1:{ cbn. case_match; try now (econstructor; eauto).
           invert_type_of_op. repeat econstructor; eauto. }
-      1:{ cbn. repeat case_match; try now (econstructor; eauto).
-          repeat invert_type_of_clear. invert_type_of_op.
-          rewrite !Bool.andb_true_iff, Bool.negb_true_iff,
-            !eqb_eq, eqb_neq in *; intuition idtac; subst.
-          repeat rewrite_map_get_put_hyp.
-          repeat clear_refl; do_injection.
+      1:{ cbn; repeat case_match; try now (econstructor; eauto);
+          repeat invert_type_of_clear; repeat invert_type_of_op_clear;
+          rewrite !Bool.andb_true_iff, !Bool.negb_true_iff,
+            !eqb_eq, !eqb_neq in *; intuition idtac; subst;
+          repeat rewrite_map_get_put_hyp;
+          repeat (repeat clear_refl; do_injection);
           repeat econstructor; eauto. }
       1:{ cbn. repeat econstructor; eauto. }
     Qed.
@@ -219,19 +297,52 @@ Section WithWord.
           rewrite IHl. f_equal. rewrite Zpos_P_of_succ_nat. case_match; auto.
           destruct p; auto. }
       1:{ repeat (case_match; auto; cbn; []).
-          rewrite !Bool.andb_true_iff, Bool.negb_true_iff, !eqb_eq, eqb_neq in *.
-          intuition idtac; subst.
-          erewrite List.fold_right_change_order;
-            [
-            | clear; intros; unfold apply_int_binop;
-              repeat case_match; auto; rewrite Z.add_shuffle3; reflexivity
-            | apply list_to_bag_to_list_Permutation ].
-          lazymatch goal with
-            H: _ = VList _ |- _ => clear H
-          end.
-          unfold get_local. induction l; cbn; auto.
-          rewrite IHl. repeat rewrite_map_get_put_goal.
-          congruence. }
+          case_match; auto; cbn; repeat (case_match; auto; cbn; []);
+          rewrite !Bool.andb_true_iff, !Bool.negb_true_iff, !eqb_eq, !eqb_neq in *;
+            intuition idtac; subst.
+          1:{ erewrite List.fold_right_change_order;
+              [
+              | clear; intros; unfold apply_int_binop;
+                repeat case_match; auto; rewrite Z.add_shuffle3; reflexivity
+              | apply list_to_bag_to_list_Permutation ].
+              lazymatch goal with
+                H: _ = VList _ |- _ => clear H
+              end.
+              unfold get_local. induction l; cbn; auto.
+              rewrite IHl. repeat rewrite_map_get_put_goal.
+              congruence. }
+          1:{ repeat invert_type_of_clear.
+              repeat invert_type_of_op_clear.
+              repeat rewrite_map_get_put_hyp.
+              repeat (repeat clear_refl; do_injection).
+            rewrite aci_aggr_alt.
+              2:{ apply_type_sound e1. rewrite_l_to_r. invert_type_of_value_clear.
+                  eauto using incl_Forall, list_to_set_incl. }
+              erewrite fold_right_change_order_idem.
+
+            2:{ intros. repeat case_match; auto; do 3 f_equal.
+                1: rewrite !Z.min_assoc;
+                rewrite (Z.min_comm z); reflexivity.
+                1: apply Z.min_comm. }
+            2:{ intros. repeat case_match; auto; do 3 f_equal.
+                1: rewrite Z.min_assoc, Z.min_id; reflexivity.
+                1: apply Z.min_id. }
+            2: apply list_to_set_incl.
+            2: apply list_to_set_incl_r.
+              eapply In_fold_right_ext with (P:=fun _ => True); auto.
+              intuition idtac; intros.
+              unfold get_local. rewrite_map_get_put_goal.
+              apply_type_sound e1. rewrite_l_to_r.
+              invert_type_of_value_clear. apply_Forall_In.
+              lazymatch goal with
+                H: type_of_value _ TInt |- _ =>
+                  inversion H; subst; clear H
+              end.
+              repeat (case_match; auto; []).
+              case_match; repeat rewrite_map_get_put_goal; auto.
+              repeat case_match; auto; f_equal;
+                unfold Z.ltb, Z.min in *; case_match;
+                rewrite ?Z.compare_eq_iff in *; congruence. } }
       1:{ case_match; auto. f_equal.
           apply Permutation_SSorted_eq;
             auto using bag_to_list_preserve_SSorted, list_to_bag_SSorted, StronglySorted_value_sort.
@@ -292,13 +403,178 @@ Section WithWord.
           auto using Permutation_list_to_bag_eq, Permutation_map, list_to_bag_to_list_Permutation. }
     Qed.
 
+    Lemma set_of_ty : forall e Gstore Genv t,
+        type_of Gstore Genv e (TList t) ->
+        type_of Gstore Genv (set_of e) (TSet t).
+    Proof.
+      induction e using expr_IH; cbn; intros.
+      all: try now (econstructor; eauto).
+      all: case_match; invert_type_of; try invert_type_of_op;
+        repeat (econstructor; eauto).
+    Qed.
+
+    Definition VSet_of (v : value) :=
+      match v with
+      | VList l => VSet (list_to_set l)
+      | _ => VUnit
+      end.
+
+    Lemma In_flat_map_incl : forall [A B : Type] (f : A -> list B) (a : A) l,
+        In a l -> incl (f a) (flat_map f l).
+    Proof.
+      induction l; cbn; intuition idtac; intros.
+      1:{ subst. apply incl_appl; apply incl_refl. }
+      1:{ apply incl_appr; assumption. }
+    Qed.
+
+    Lemma incl_flat_map : forall [A B : Type] (f : A -> list B) [l1 l2 : list A],
+        incl l1 l2 -> incl (flat_map f l1) (flat_map f l2).
+    Proof.
+      induction l1; cbn; auto using incl_nil_l.
+      intros. apply incl_cons_inv in H; intuition idtac.
+      apply incl_app; auto using In_flat_map_incl.
+    Qed.
+
+    Lemma flat_map_incl_in : forall [A B : Type] (f g : A -> list B) [l : list A],
+      (forall a, In a l -> incl (f a) (g a)) ->
+      incl (flat_map f l) (flat_map g l).
+    Proof.
+      induction l; cbn; auto using incl_refl; intros.
+      apply incl_app_app; auto.
+    Qed.
+
+    Lemma flat_map_incl_in2 : forall [A B : Type] (f g : A -> list B) [l1 l2 : list A],
+        incl l1 l2 ->
+        (forall a, In a l2 -> incl (f a) (g a)) ->
+        incl (flat_map f l1) (flat_map g l2).
+    Proof.
+      induction l1; cbn; auto using incl_nil_l; intros.
+      apply incl_cons_inv in H; intuition idtac.
+      apply incl_app; auto.
+      eapply incl_tran; [ apply In_flat_map_incl | ]; eauto using flat_map_incl_in.
+    Qed.
+
+    Lemma NoDup_SSorted_double_incl_eq : forall (l1 l2 : list value),
+        NoDup l1 -> NoDup l2 ->
+        StronglySorted value_leb l1 ->
+        StronglySorted value_leb l2 ->
+        incl l1 l2 -> incl l2 l1 ->
+        l1 = l2.
+    Proof.
+      induction l1; intros.
+      1: apply incl_l_nil in H4; congruence.
+      destruct l2.
+      1:{ unfold incl in *.
+          lazymatch goal with
+            H: forall _, In _ (?a :: _) -> _ |- _ =>
+              specialize (H a) end.
+          cbn in *. intuition fail. }
+      1:{
+        repeat lazymatch goal with
+        | H: NoDup (_ :: _) |- _ => inversion H; clear H
+          | H: StronglySorted _ (_ :: _) |- _ => inversion H; clear H
+          | H: incl (_ :: _) _ |- _ => apply incl_cons_inv in H
+          end; subst.
+        intuition idtac.
+        assert (a = v).
+        { destruct (value_eqb a v) eqn:E.
+          1: apply value_eqb_eq in E; congruence.
+          apply value_eqb_neq in E.
+          lazymatch goal with
+            H: In a (v :: _), H': In v (a :: _) |- _ =>
+              inversion H; inversion H' end;
+          auto. repeat apply_Forall_In.
+          apply value_leb_antisym; auto. }
+        f_equal; auto; subst.
+        1:{ apply IHl1; auto;
+            unfold incl in *; intros;
+            lazymatch goal with
+              H: forall _, In _ ?l1 -> In _ (_ :: ?l2),
+              H': In _ ?l1 |- In _ ?l2 =>
+              apply H in H' as H_in end;
+            destruct (value_eqb a v) eqn:E;
+            try (apply value_eqb_eq in E; subst; intuition idtac);
+            inversion H_in; auto;
+            apply value_eqb_neq in E; congruence. } }
+    Qed.
+
+    Lemma incl_filter_incl : forall [A : Type] (f : A -> bool) (l1 l2 : list A),
+        incl l1 l2 ->
+        incl (filter f l1) (filter f l2).
+    Proof.
+      induction l1; cbn; auto using incl_nil_l; intros.
+      apply incl_cons_inv in H.
+      case_match; intuition auto.
+      apply incl_cons; auto.
+      rewrite filter_In; auto.
+    Qed.
+
+    Ltac use_set_of_sem_IH :=
+      lazymatch goal with
+        IH: context[interp_expr _ _ (set_of ?e)] |- context[interp_expr _ _ (set_of ?e)] =>
+          rewrite IH; clear IH end.
+
+    Lemma set_of_sem : forall e (Gstore Genv : tenv) t,
+        type_of Gstore Genv e (TList t) ->
+        forall (store env : locals),
+        tenv_wf Gstore -> tenv_wf Genv ->
+        locals_wf Gstore store -> locals_wf Genv env ->
+        interp_expr store env (set_of e) = VSet_of (interp_expr store env e).
+    Proof.
+      induction 1; unfold VSet_of in *; auto; intros.
+      1:{ cbn. case_match; auto; cbn; use_set_of_sem_IH; auto.
+          case_match; auto. }
+      1:{ cbn. use_set_of_sem_IH; auto.
+          case_match; auto. f_equal.
+          apply NoDup_SSorted_double_incl_eq; auto using list_to_set_NoDup, list_to_set_SSorted.
+          1:{ eapply incl_tran; [ apply list_to_set_incl | ].
+              eapply incl_tran; [ apply incl_flat_map, list_to_set_incl | ].
+              eapply incl_tran; [ | apply list_to_set_incl_r ].
+              apply flat_map_incl_in; intros.
+              apply_type_sound e1. rewrite_l_to_r.
+              invert_type_of_value_clear. apply_Forall_In.
+              rewrite IHtype_of2; eauto with fiat2_hints.
+              case_match; auto using incl_refl, list_to_set_incl. }
+          1:{ eapply incl_tran; [ | apply list_to_set_incl_r ].
+              eapply incl_tran; [ | apply incl_flat_map, list_to_set_incl_r ].
+              eapply incl_tran; [ apply list_to_set_incl | ].
+              apply flat_map_incl_in; intros.
+              apply_type_sound e1. rewrite_l_to_r.
+              invert_type_of_value_clear. apply_Forall_In.
+              rewrite IHtype_of2; eauto with fiat2_hints.
+              case_match; auto using incl_refl, list_to_set_incl_r. } }
+      1:{ cbn. use_set_of_sem_IH; auto.
+          case_match; auto. f_equal.
+          apply NoDup_SSorted_double_incl_eq; auto using list_to_set_NoDup, list_to_set_SSorted, NoDup_filter, filter_preserve_SSorted;
+            eauto using incl_tran, list_to_set_incl_r,
+            incl_filter_incl, list_to_set_incl. }
+      1:{ cbn. use_set_of_sem_IH; auto.
+          case_match; auto.
+          use_set_of_sem_IH; auto.
+          case_match; auto. f_equal.
+          apply NoDup_SSorted_double_incl_eq; auto using list_to_set_NoDup, list_to_set_SSorted, NoDup_filter, filter_preserve_SSorted.
+          1:{ eapply incl_tran; [ apply list_to_set_incl | ].
+              eapply incl_tran; [ | apply list_to_set_incl_r ].
+              apply flat_map_incl_in2; [ apply list_to_set_incl | ].
+              intros. apply incl_map, incl_filter_incl, list_to_set_incl. }
+          1:{ eapply incl_tran; [ apply list_to_set_incl | ].
+              eapply incl_tran; [ | apply list_to_set_incl_r ].
+              apply flat_map_incl_in2; [ apply list_to_set_incl_r | ].
+              intros. apply incl_map, incl_filter_incl, list_to_set_incl_r. } }
+      1:{ cbn. use_set_of_sem_IH; auto.
+          case_match; auto. f_equal.
+          apply NoDup_SSorted_double_incl_eq; auto using list_to_set_NoDup, list_to_set_SSorted;
+            eauto using incl_tran, list_to_set_incl_r,
+            incl_map, list_to_set_incl. }
+    Qed.
+
     Theorem push_down_collection_preserve_ty : forall e Gstore Genv t,
         type_of Gstore Genv e t ->
         type_of Gstore Genv (push_down_collection e) t.
     Proof.
       destruct 1.
       all: try now (econstructor; eauto).
-      cbn. auto using bag_of_ty.
+      all: cbn; auto using bag_of_ty, set_of_ty.
     Qed.
 
     Theorem push_down_collection_preserve_sem : forall e (Gstore Genv : tenv) t (store env : locals),
@@ -308,7 +584,8 @@ Section WithWord.
         interp_expr store env (push_down_collection e) = interp_expr store env e.
     Proof.
       destruct 1; auto; cbn; intros.
-      erewrite bag_of_sem; eauto.
+      1: erewrite bag_of_sem; eauto.
+      1: erewrite set_of_sem; eauto.
     Qed.
 
     Theorem push_down_collection_sound : expr_transf_sound (locals:=locals) push_down_collection.
